added function to abstract state

AbstractAnalysis.v
@@ -5,7 +5,7 @@ Inductive info : Set :=
 | unbounded
 | mem_bounded
 | cf_bounded
-| heap_base.
+| mem_base.
 
 Definition abs_registers_ty := fmap register info.
 
@@ -16,15 +16,15 @@ Definition abs_stack_ty := list info.
 (* Definition flags_ty := fmap flag abs_state. *)
 
 Record abs_state := {
-  regs : abs_registers_ty;
+  abs_regs : abs_registers_ty;
 (*  flags : flags_ty; *)
-  stack : abs_stack_ty;
+  abs_stack : abs_stack_ty;
 (*  heap : heap_ty; *)
 }.
 
 Definition abs_empty_abs_state :=
-{| regs := fun r => if register_eq_dec r rdi then heap_base else unbounded;
-   stack := nil;
+{| abs_regs := fun r => if register_eq_dec r rdi then mem_base else unbounded;
+   abs_stack := nil;
 (*   heap := nil *)|}.
 
 (*
@@ -37,7 +37,7 @@ Inductive value : Set :=
 (*
 Fixpoint value_to_word64 (s : machine) (v :value) : word64 :=
 match v with
-| A_Reg r => (regs s) r
+| A_Reg r => (abs_regs s) r
 | A_Const c => c
 | A_MultPlus m v1 v2 => wmult m (wplus (value_to_word64 s v1) (value_to_word64 s v2))
 end.
@@ -45,38 +45,38 @@ end.
 
 (*
 Definition read_register (s : machine) (r : register) : word64 :=
-  get register word64 s.(regs) r.
+  get register word64 s.(abs_regs) r.
 *)
 
 (*
 Definition write_register (s : machine) (r : register) (v : word64) : machine :=
-{| regs := set register register_eq_dec word64 s.(regs) r v;
+{| abs_regs := set register register_eq_dec word64 s.(abs_regs) r v;
    flags := s.(flags);
-   stack := s.(stack);
+   abs_stack := s.(stack);
    heap := s.(heap) |}.
 *)
 
 (*
 Definition set_flags (s : machine) (f : flags_ty) : machine :=
-{| regs := s.(regs);
+{| abs_regs := s.(abs_regs);
    flags := f;
-   stack := s.(stack);
+   abs_stack := s.(stack);
    heap := s.(heap) |}. 
 *)
 
-Definition expand_stack (s : abs_state) (i : nat) : abs_state :=
-{| regs := s.(regs);
+Definition expand_abs_stack (s : abs_state) (i : nat) : abs_state :=
+{| abs_regs := s.(abs_regs);
 (*   flags := s.(flags); *)
-   stack := s.(stack) ++ (repeat unbounded i);
+   abs_stack := s.(abs_stack) ++ (repeat unbounded i);
 (*   heap := s.(heap) *)|}.
 
-Fixpoint contract_stack (s : abs_state) (i : nat) : abs_state :=
+Fixpoint contract_abs_stack (s : abs_state) (i : nat) : abs_state :=
 match i with
 | 0 => s
 | S n =>
-contract_stack {| regs := s.(regs);
+contract_abs_stack {| abs_regs := s.(abs_regs);
 (*   flags := s.(flags); *)
-   stack := removelast s.(stack);
+   abs_stack := removelast s.(abs_stack);
 (*   heap := s.(heap) *) |} n
 end.
 
@@ -89,10 +89,10 @@ end.
 *)
 
 (*
-Program Fixpoint read_stack (s : machine) (i : nat) (sz : nat) : word (8 * sz):=
+Program Fixpoint read_abs_stack (s : machine) (i : nat) (sz : nat) : word (8 * sz):=
 match sz with
 | 0 => WO
-| S sz' => combine (read_stack_word s i) (read_stack s (i+1) (sz'))
+| S sz' => combine (read_stack_word s i) (read_abs_stack s (i+1) (sz'))
 end.
 Next Obligation. rewrite <- plus_n_O. repeat (rewrite <- plus_n_Sm). reflexivity.
 Qed.
@@ -114,20 +114,20 @@ Qed.
 *)
 
 Definition get_register_info (s : abs_state) (r : register) : info :=
-  map_get s.(regs) r.
+  map_get s.(abs_regs) r.
 
 Definition set_register_info (s : abs_state) (r : register) (i : info) : abs_state :=
-{| regs := map_set register_eq_dec s.(regs) r i;
-   stack := s.(stack);
+{| abs_regs := map_set register_eq_dec s.(abs_regs) r i;
+   abs_stack := s.(abs_stack);
 (*   heap := s.(heap) *) |}.
 
 Definition get_stack_info (s : abs_state) (index : nat) : info :=
-nth index s.(stack) unbounded.
+nth index s.(abs_stack) unbounded.
 
 (* this needs to be updated *)
 Definition set_stack_info (s : abs_state) (index : nat) (i : info) : abs_state :=
-{| regs := s.(regs);
-   stack := update s.(stack) index i;
+{| abs_regs := s.(abs_regs);
+   abs_stack := update s.(abs_stack) index i;
  (*  heap := s.(heap) *) |}.
 
 Definition empty {A} (l : list A) :=
@@ -138,12 +138,12 @@ Reserved Notation " st '|-' i '⟶' st' "
 Inductive instr_class_flow_function : instr_class -> abs_state -> abs_state -> Prop := 
 | I_Heap_Read: forall st r_base r_src r_dst,
     (* r_base <> r_src -> *) (* not sure if we need this to make the proofs easier *)
-    get_register_info st r_base = heap_base ->
+    get_register_info st r_base = mem_base ->
     get_register_info st r_src = mem_bounded ->
     st |- (Heap_Read r_dst r_src r_base) ⟶ (set_register_info st r_dst unbounded) 
 | I_Heap_Write: forall st r_base r_src r_dst,
     (* r_base <> r_src -> *) (* not sure if we need this to make the proofs easier *)
-    get_register_info st r_base = heap_base ->
+    get_register_info st r_base = mem_base ->
     get_register_info st r_src = mem_bounded -> 
     st |- (Heap_Write r_dst r_src r_base) ⟶ st
 | I_Heap_Check: forall st r_src,
@@ -155,24 +155,24 @@ Inductive instr_class_flow_function : instr_class -> abs_state -> abs_state -> P
 | I_Reg_Write: forall st r_dst val,
     st |- (Reg_Write r_dst val) ⟶ (set_register_info st r_dst unbounded)
 | I_Stack_Expand: forall st i,
-    st |- (Stack_Expand i) ⟶ (expand_stack st i)
+    st |- (Stack_Expand i) ⟶ (expand_abs_stack st i)
 | I_Stack_Contract: forall st i,
-    st |- (Stack_Contract i) ⟶ (contract_stack st i)
+    st |- (Stack_Contract i) ⟶ (contract_abs_stack st i)
 | I_Stack_Read: forall st i r_dst,
-    i < (length st.(stack)) ->
+    i < (length st.(abs_stack)) ->
     st |- (Stack_Read r_dst i) ⟶ (set_register_info st r_dst (get_stack_info st i))
 | I_Stack_Write: forall st i r_src,
-    i < (length st.(stack)) ->
+    i < (length st.(abs_stack)) ->
     st |- (Stack_Write i r_src) ⟶ (set_stack_info st i (get_register_info st r_src))
 | I_Indirect_Call: forall st reg,
     get_register_info st reg = cf_bounded ->
-    get_register_info st rdi = heap_base ->
+    get_register_info st rdi = mem_base ->
     st |- (Indirect_Call reg) ⟶  st
 | I_Direct_Call: forall st,
-    get_register_info st rdi = heap_base ->
+    get_register_info st rdi = mem_base ->
     st |- (Direct_Call) ⟶  st
 | I_Ret: forall st,
-    empty st.(stack) ->
+    empty st.(abs_stack) ->
     st |- (Ret) ⟶  st
   where " st '|-' i '⟶' st' " := (instr_class_flow_function i st st').
 
@@ -187,29 +187,29 @@ Record cfg_ty := {
   edges : list (basic_block * basic_block)
 }.
 
-Lemma register_get_after_set_eq : forall (regs : abs_registers_ty) reg v,
-    map_get (map_set register_eq_dec regs reg v) reg = v.
+Lemma register_get_after_set_eq : forall (abs_regs : abs_registers_ty) reg v,
+    map_get (map_set register_eq_dec abs_regs reg v) reg = v.
 Proof.
-  intros regs reg v. unfold map_get. unfold map_set. destruct (register_eq_dec reg reg).
+  intros abs_regs reg v. unfold map_get. unfold map_set. destruct (register_eq_dec reg reg).
   - reflexivity.
   - exfalso. apply n. reflexivity.
 Qed.
 
-Lemma register_get_after_set_neq : forall (regs : abs_registers_ty) reg1 reg2 v,
+Lemma register_get_after_set_neq : forall (abs_regs : abs_registers_ty) reg1 reg2 v,
     reg1 <> reg2 ->
-    map_get (map_set register_eq_dec regs reg2 v) reg1 = map_get regs reg1.
+    map_get (map_set register_eq_dec abs_regs reg2 v) reg1 = map_get abs_regs reg1.
 Proof.
-  intros regs reg1 reg2 v Heq. unfold map_get. unfold map_set. destruct (register_eq_dec reg2 reg1).
+  intros abs_regs reg1 reg2 v Heq. unfold map_get. unfold map_set. destruct (register_eq_dec reg2 reg1).
   - exfalso. apply Heq. auto.
   - reflexivity.
 Qed.
 
 Definition safe_stack_read (st : abs_state) (r_base : register) (r_src : register) (r_dst : register) : Prop :=
-  r_base <> r_src /\ get_register_info st r_base = heap_base /\ get_register_info st r_src = mem_bounded.
+  r_base <> r_src /\ get_register_info st r_base = mem_base /\ get_register_info st r_src = mem_bounded.
 
 Lemma read_after_check_is_safe: forall r_base r_src r_dst st, exists st' st'',
   r_base <> r_src ->
-  get_register_info st r_base = heap_base ->
+  get_register_info st r_base = mem_base ->
   st |- (Heap_Check r_src) ⟶ st' /\ st' |- (Heap_Read r_dst r_src r_base) ⟶ st''.
 Proof.
   intros r_base r_src r_dst st. 
