Safety.v
@@ -2,8 +2,12 @@ Require Import Semantics.
 Require Import Machine.
 Require Import Bits.
 Require Import Coq.Init.Nat.
+Require Import Coq.Lists.List.
 Require Import Coq.Lists.ListSet.
 Require Import AbstractAnalysis.
+
+Definition member (s : set int64) (i : int64) :=
+  set_mem int64_eq_dec i s.
 
 Definition is_mem_bounded (s : state) (r_src : register) (r_base : register) : bool :=
   andb (Word.eq (get_register s r_base) s.(heap_base)) (Word.lt (get_register s r_src) fourGB).
@@ -21,7 +25,7 @@ Definition is_rdi_heapbase (s : state) : bool :=
   Word.eq (get_register s rdi) s.(heap_base).
 
 Definition is_function_index_safe (s : state) (r : register) : bool :=
-  set_mem int64_eq_dec (get_register s r) s.(function_table).
+  member s.(function_table) (get_register s r).
 
 Definition is_instr_class_safe (s : state) (i : instr_class) : bool :=
   match i with
@@ -36,7 +40,24 @@ Definition is_instr_class_safe (s : state) (i : instr_class) : bool :=
 | _ => true
 end.
 
+Definition abstractify_int64 (s : state) (i : int64) : info :=
+if (Word.eq i s.(heap_base)) then mem_base else
+if (member s.(function_table) i) then cf_bounded else
+if (Word.lt i fourGB) then mem_bounded else unbounded.
+
+Definition abstractify_list (s : state) (l : list int64) : list info :=
+  map (abstractify_int64 s) l.
+
+Definition abstractify_registers (s : state) (f : registers_ty) : abs_registers_ty :=
+  fun r => (abstractify_int64 s (f r)).
+
+Definition abstractify (s : state) : abs_state :=
+{| abs_regs := abstractify_registers s s.(regs);
+   abs_stack := abstractify_list s s.(stack) |}.
+
 Theorem safe_instr : 
   forall i st,
-    exists st', instr_class_flow_function i st st' ->
+    exists st', instr_class_flow_function i (abstractify st) (abstractify st') ->
     is_instr_class_safe st i = true.
+Proof.
+  intros i st. eexists st'. induction i.
